#+OPTIONS: author:nil ^:{}
#+HUGO_FRONT_MATTER_FORMAT: YAML
#+HUGO_BASE_DIR: ~/blog/
#+HUGO_SECTION: posts
#+DATE:<2023-11-29 Wed>
#+HUGO_CUSTOM_FRONT_MATTER: :toc true
#+HUGO_AUTO_SET_LASTMOD: t
#+HUGO_TAGS: "Advanced Algebra"
#+HUGO_DRAFT: false
#+TITLE: Fibonacci numbers and determinant
Fibonacci sequence is a sequence as

$$1, 2, 3, 5, 8, 13, 21, 34, \cdots,$$

it satisfies: $F_n = F_{n - 1} + F_{n - 2}(n \ge 3), F_1 = 1, F_2 = 2$

1. Proof the Fibonacci numbers $F_n$ can be get from the determinant
   \[
   F_n =
   {\begin{vmatrix}
   1 & -1 & 0 & 0 & \cdots & 0 & 0 & 0\\
   1 & 1 & -1 & 0 & \cdots & 0 & 0 & 0\\
   0 & 1 & 1 & -1 & \cdots & 0 & 0 & 0\\
   \vdots & \vdots & \vdots & \vdots & & \vdots & \vdots & \vdots\\
   0 & 0 & 0 & 0 & \cdots & 1 & 1 & -1\\
   0 & 0 & 0 & 0 & \cdots & 0 & 1 & 1\\
   \end{vmatrix} };
   \]

   #+BEGIN_PROOF
   Use induction can proof it.
   #+END_PROOF
2. Show the formula of Fibonacci numbers

   Because $F_n = F_{n - 1} + F_{n - 2}(n \ge 3), F_1 = 1, F_2 = 2$, suppose
   $$F_n - aF_{n - 1} = b(F_{n - 1} - aF_{n - 2})$$
   so
   $$F_n = (a + b)F_{n - 1} - abF_{n - 2}$$
   $$F_n - bF_{n - 1} = a(F_{n - 1} - bF_{n - 2})$$
   then we get $a + b = 1, ab = -1$, so
   $$a = \frac{1 + \sqrt{5}}{2}, b = \frac{1 - \sqrt{5}}{2}$$
   or
   $$a = \frac{1 - \sqrt{5}}{2}, b = \frac{1 + \sqrt{5}}{2}$$
   we consider the first case, because $F_2 = 2, F_1 = 1$, so
   $$F_n - aF_{n - 1} = b^{n - 2}(2 - a) = b^{n - 2}(1 + b) = b^{n - 2} + b^{n - 1}$$
   $$F_n - bF_{n - 1} = a^{n - 2}(2 - b) = a^{n - 2}(1 + a) = a^{n - 2} + a^{n - 1}$$
   so
   $$F_n = \frac{a^{n} + a^{n - 1} - b^{n} - b^{n - 1}}{a - b}$$
   because $ab = -1$, we can get a more elegant conclusion
   $$F_n = \frac{a^{n + 1} - b^{n + 1}}{a - b}$$
